disk-betree/ImplState.dfy
@@ -1,0 +1,103 @@
+include "PivotBetreeSpec.dfy"
+include "Message.dfy"
+include "../lib/Option.dfy"
+include "SSTable.dfy"
+include "BetreeBlockCache.dfy"
+
+module ImplState {
+  import opened Options
+  import opened Sequences
+
+  import BT = PivotBetreeSpec`Internal
+  import Messages = ValueMessage
+  import MS = MapSpec
+  import Pivots = PivotsLib
+  import BC = BetreeGraphBlockCache
+  import M = BetreeBlockCache
+  import SSTable = SSTable
+
+  type Reference = BT.G.Reference
+  type Key = MS.Key
+  type Message = Messages.Message
+
+  datatype Node = Node(
+      pivotTable: Pivots.PivotTable,
+      children: Option<seq<Reference>>,
+      buckets: seq<SSTable.SSTable>
+    )
+  datatype Variables =
+    | Ready(
+        persistentSuperblock: BC.Superblock,
+        ephemeralSuperblock: BC.Superblock,
+        cache: map<Reference, Node>)
+    | Unready
+  datatype Sector =
+    | SectorBlock(block: Node)
+    | SectorSuperblock(superblock: BC.Superblock)
+
+  predicate WFBuckets(buckets: seq<SSTable.SSTable>)
+  {
+    forall i | 0 <= i < |buckets| :: SSTable.WFSSTableMap(buckets[i])
+  }
+  predicate WFNode(node: Node)
+  {
+    WFBuckets(node.buckets)
+  }
+  predicate WFCache(cache: map<Reference, Node>)
+  {
+    forall ref | ref in cache :: WFNode(cache[ref])
+  }
+  predicate WFVars(vars: Variables)
+  {
+    match vars {
+      case Ready(persistentSuperblock, ephemeralSuperblock, cache) => WFCache(cache)
+      case Unready => true
+    }
+  }
+  predicate WFSector(sector: Sector)
+  {
+    match sector {
+      case SectorBlock(node) => WFNode(node)
+      case SectorSuperblock(superblock) => BC.WFPersistentSuperblock(superblock)
+    }
+  }
+
+  function IBuckets(buckets: seq<SSTable.SSTable>) : seq<map<Key, Message>>
+  requires WFBuckets(buckets)
+  {
+    if |buckets| == 0 then [] else IBuckets(DropLast(buckets)) + [SSTable.I(Last(buckets))]
+  }
+  function INode(node: Node) : BT.G.Node
+  requires WFNode(node)
+  {
+    BT.G.Node(node.pivotTable, node.children, IBuckets(node.buckets))
+  }
+  function ICache(cache: map<Reference, Node>) : map<Reference, BT.G.Node>
+  requires WFCache(cache)
+  {
+    map ref | ref in cache :: INode(cache[ref])
+  }
+  function IVars(vars: Variables) : M.Variables
+  requires WFVars(vars)
+  {
+    match vars {
+      case Ready(persistentSuperblock, ephemeralSuperblock, cache) =>
+        BC.Ready(persistentSuperblock, ephemeralSuperblock, ICache(cache))
+      case Unready => BC.Unready
+    }
+  }
+
+  class ImplHeapState {
+    var s: Variables
+    constructor()
+    ensures WFVars(s)
+    ensures M.Init(BC.Constants(), IVars(s));
+    {
+      s := Unready;
+    }
+  }
+  type HeapState = ImplHeapState
+  function HeapSet(hs: HeapState) : set<object> { {hs} }
+
+  
+}
